Coercions into values.

lib.v
@@ -1,7 +1,16 @@
 From stdpp Require Import base countable gmap.
+From iris.heap_lang Require Import lang notation.
 
 Definition perm `{!EqDecision T, !Countable T} (X : gset (T * T)) :=
   forall p1 p2, p1 ∈ X → p2 ∈ X → (p1.1 = p2.1 ↔ p1.2 = p2.2).
 
 Definition flipb {T S} (b : bool) (f : T → T → S) x y :=
   f (if b then x else y) (if b then y else x).
+
+Class AsVal A := as_val : A -> val.
+
+Instance as_val_option `{AsVal A} : AsVal (option A) := λ x,
+  match x with
+  | Some x => SOMEV (as_val x)
+  | None => NONEV
+  end.
